src/QUIC.Impl.fst
@@ -1,11 +1,10 @@
 module QUIC.Impl
 
-(*
 // This MUST be kept in sync with QUIC.Impl.fsti...
 module G = FStar.Ghost
 module B = LowStar.Buffer
 module IB = LowStar.ImmutableBuffer
-module S = FStar.Seq
+module Seq = QUIC.Secret.Seq
 module HS = FStar.HyperStack
 module ST = FStar.HyperStack.ST
 
@@ -54,7 +53,7 @@ type state_s (i: index) =
       aead_state:EverCrypt.AEAD.state the_aead_alg ->
       iv:EverCrypt.AEAD.iv_p the_aead_alg ->
       hp_key:B.buffer U8.t { B.length hp_key = QUIC.Spec.ae_keysize the_aead_alg } ->
-      pn:B.pointer u62 ->
+      pn:B.pointer PN.packet_number_t ->
       ctr_state:CTR.state (as_cipher_alg the_aead_alg) ->
       state_s i
 
@@ -87,10 +86,10 @@ let invariant_s #i h s =
   B.(all_disjoint [ CTR.footprint h ctr_state;
     AEAD.footprint h aead_state; loc_buffer iv; loc_buffer hp_key; loc_buffer pn ]) /\
   // JP: automatic insertion of reveal does not work here
-  G.reveal initial_pn <= U64.v (B.deref h pn) /\
-  AEAD.as_kv (B.deref h aead_state) ==
+  G.reveal initial_pn <= Secret.v (B.deref h pn) /\
+  Seq.seq_reveal (AEAD.as_kv (B.deref h aead_state)) ==
     derive_secret i.hash_alg (G.reveal traffic_secret) label_key (Spec.Agile.AEAD.key_length aead_alg) /\
-  B.as_seq h iv ==
+  Seq.seq_reveal (B.as_seq h iv) ==
     derive_secret i.hash_alg (G.reveal traffic_secret) label_iv 12 /\
   B.as_seq h hp_key ==
     derive_secret i.hash_alg (G.reveal traffic_secret) label_hp (QUIC.Spec.ae_keysize aead_alg)
@@ -167,12 +166,12 @@ let op_inplace (dst: B.buffer U8.t)
       B.length dst >= U32.v ofs + B.length src)
     (ensures fun h0 _ h1 ->
       B.(modifies (loc_buffer dst) h0 h1) /\
-      B.as_seq h1 dst `S.equal`
+      B.as_seq h1 dst `Seq.equal`
         QUIC.Spec.Lemmas.pointwise_op op (B.as_seq h0 dst) (B.as_seq h0 src) (U32.v ofs) /\
-      S.slice (B.as_seq h0 dst) 0 (U32.v ofs) `S.equal`
-        S.slice (B.as_seq h1 dst) 0 (U32.v ofs) /\
-      S.slice (B.as_seq h0 dst) (U32.v (ofs `U32.add` src_len)) (U32.v dst_len) `S.equal`
-      S.slice (B.as_seq h1 dst) (U32.v (ofs `U32.add` src_len)) (U32.v dst_len))
+      Seq.slice (B.as_seq h0 dst) 0 (U32.v ofs) `Seq.equal`
+        Seq.slice (B.as_seq h1 dst) 0 (U32.v ofs) /\
+      Seq.slice (B.as_seq h0 dst) (U32.v (ofs `U32.add` src_len)) (U32.v dst_len) `Seq.equal`
+      Seq.slice (B.as_seq h1 dst) (U32.v (ofs `U32.add` src_len)) (U32.v dst_len))
 =
   let h0 = ST.get () in
   let dst0 = B.sub dst 0ul ofs in
@@ -180,51 +179,51 @@ let op_inplace (dst: B.buffer U8.t)
   let dst2 = B.sub dst (ofs `U32.add` src_len) (dst_len `U32.sub` (ofs `U32.add` src_len)) in
   C.Loops.in_place_map2 dst1 src src_len op;
   let h1 = ST.get () in
-  calc (S.equal) {
+  calc (Seq.equal) {
     B.as_seq h1 dst;
-  (S.equal) { lemma_slice3 (B.as_seq h1 dst) (U32.v ofs) (U32.v (ofs `U32.add` src_len)) }
-    S.slice (B.as_seq h1 dst) 0 (U32.v ofs) `S.append`
-    (S.slice (B.as_seq h1 dst) (U32.v ofs) (U32.v (ofs `U32.add` src_len))) `S.append`
-    (S.slice (B.as_seq h1 dst) (U32.v (ofs `U32.add` src_len)) (B.length dst));
-  (S.equal) {}
-    S.slice (B.as_seq h0 dst) 0 (U32.v ofs) `S.append`
-    (S.slice (B.as_seq h1 dst) (U32.v ofs) (U32.v (ofs `U32.add` src_len))) `S.append`
-    (S.slice (B.as_seq h0 dst) (U32.v (ofs `U32.add` src_len)) (B.length dst));
-  (S.equal) { pointwise_seq_map2 op (B.as_seq h0 dst1) (B.as_seq h0 src) 0 }
-    S.slice (B.as_seq h0 dst) 0 (U32.v ofs) `S.append`
+  (Seq.equal) { lemma_slice3 (B.as_seq h1 dst) (U32.v ofs) (U32.v (ofs `U32.add` src_len)) }
+    Seq.slice (B.as_seq h1 dst) 0 (U32.v ofs) `Seq.append`
+    (Seq.slice (B.as_seq h1 dst) (U32.v ofs) (U32.v (ofs `U32.add` src_len))) `Seq.append`
+    (Seq.slice (B.as_seq h1 dst) (U32.v (ofs `U32.add` src_len)) (B.length dst));
+  (Seq.equal) {}
+    Seq.slice (B.as_seq h0 dst) 0 (U32.v ofs) `Seq.append`
+    (Seq.slice (B.as_seq h1 dst) (U32.v ofs) (U32.v (ofs `U32.add` src_len))) `Seq.append`
+    (Seq.slice (B.as_seq h0 dst) (U32.v (ofs `U32.add` src_len)) (B.length dst));
+  (Seq.equal) { pointwise_seq_map2 op (B.as_seq h0 dst1) (B.as_seq h0 src) 0 }
+    Seq.slice (B.as_seq h0 dst) 0 (U32.v ofs) `Seq.append`
     (QUIC.Spec.Lemmas.pointwise_op op
-      (S.slice (B.as_seq h0 dst) (U32.v ofs) (U32.v (ofs `U32.add` src_len)))
+      (Seq.slice (B.as_seq h0 dst) (U32.v ofs) (U32.v (ofs `U32.add` src_len)))
       (B.as_seq h0 src)
-      0) `S.append`
-    (S.slice (B.as_seq h0 dst) (U32.v (ofs `U32.add` src_len)) (B.length dst));
-  (S.equal) { QUIC.Spec.Lemmas.pointwise_op_suff op (S.slice (B.as_seq h0 dst) 0 (U32.v ofs))
-    (S.slice (B.as_seq h0 dst) (U32.v ofs) (U32.v (ofs `U32.add` src_len)))
+      0) `Seq.append`
+    (Seq.slice (B.as_seq h0 dst) (U32.v (ofs `U32.add` src_len)) (B.length dst));
+  (Seq.equal) { QUIC.Spec.Lemmas.pointwise_op_suff op (Seq.slice (B.as_seq h0 dst) 0 (U32.v ofs))
+    (Seq.slice (B.as_seq h0 dst) (U32.v ofs) (U32.v (ofs `U32.add` src_len)))
     (B.as_seq h0 src)
     (U32.v ofs) }
     QUIC.Spec.Lemmas.pointwise_op op
-      (S.append (S.slice (B.as_seq h0 dst) 0 (U32.v ofs))
-        (S.slice (B.as_seq h0 dst) (U32.v ofs) (U32.v (ofs `U32.add` src_len))))
+      (Seq.append (Seq.slice (B.as_seq h0 dst) 0 (U32.v ofs))
+        (Seq.slice (B.as_seq h0 dst) (U32.v ofs) (U32.v (ofs `U32.add` src_len))))
       (B.as_seq h0 src)
-      (U32.v ofs) `S.append`
-    (S.slice (B.as_seq h0 dst) (U32.v (ofs `U32.add` src_len)) (B.length dst));
-  (S.equal) { lemma_slice1 (B.as_seq h0 dst) (U32.v ofs) (U32.v (ofs `U32.add` src_len)) }
+      (U32.v ofs) `Seq.append`
+    (Seq.slice (B.as_seq h0 dst) (U32.v (ofs `U32.add` src_len)) (B.length dst));
+  (Seq.equal) { lemma_slice1 (B.as_seq h0 dst) (U32.v ofs) (U32.v (ofs `U32.add` src_len)) }
     QUIC.Spec.Lemmas.pointwise_op op
-      (S.slice (B.as_seq h0 dst) 0 (U32.v (ofs `U32.add` src_len)))
+      (Seq.slice (B.as_seq h0 dst) 0 (U32.v (ofs `U32.add` src_len)))
       (B.as_seq h0 src)
-      (U32.v ofs) `S.append`
-    (S.slice (B.as_seq h0 dst) (U32.v (ofs `U32.add` src_len)) (B.length dst));
-  (S.equal) { QUIC.Spec.Lemmas.pointwise_op_pref op
-    (S.slice (B.as_seq h0 dst) 0 (U32.v (ofs `U32.add` src_len)))
-    (S.slice (B.as_seq h0 dst) (U32.v (ofs `U32.add` src_len)) (B.length dst))
+      (U32.v ofs) `Seq.append`
+    (Seq.slice (B.as_seq h0 dst) (U32.v (ofs `U32.add` src_len)) (B.length dst));
+  (Seq.equal) { QUIC.Spec.Lemmas.pointwise_op_pref op
+    (Seq.slice (B.as_seq h0 dst) 0 (U32.v (ofs `U32.add` src_len)))
+    (Seq.slice (B.as_seq h0 dst) (U32.v (ofs `U32.add` src_len)) (B.length dst))
     (B.as_seq h0 src)
     (U32.v ofs)
   }
     QUIC.Spec.Lemmas.pointwise_op op
-      (S.slice (B.as_seq h0 dst) 0 (U32.v (ofs `U32.add` src_len)) `S.append`
-      (S.slice (B.as_seq h0 dst) (U32.v (ofs `U32.add` src_len)) (B.length dst)))
+      (Seq.slice (B.as_seq h0 dst) 0 (U32.v (ofs `U32.add` src_len)) `Seq.append`
+      (Seq.slice (B.as_seq h0 dst) (U32.v (ofs `U32.add` src_len)) (B.length dst)))
       (B.as_seq h0 src)
       (U32.v ofs);
-  (S.equal) { lemma_slice (B.as_seq h0 dst) (U32.v (ofs `U32.add` src_len)) }
+  (Seq.equal) { lemma_slice (B.as_seq h0 dst) (U32.v (ofs `U32.add` src_len)) }
     QUIC.Spec.Lemmas.pointwise_op op
       (B.as_seq h0 dst)
       (B.as_seq h0 src)
@@ -252,7 +251,7 @@ val derive_secret: a: QUIC.Spec.ha ->
       assert_norm (255 < pow2 61);
       assert_norm (pow2 61 < pow2 125);
       B.(modifies (loc_buffer dst) h0 h1) /\
-      B.as_seq h1 dst == QUIC.Spec.derive_secret a (B.as_seq h0 secret)
+      B.as_seq h1 dst == QUIC.Spec.derive_secret a (Seq.seq_hide (B.as_seq h0 secret))
         (IB.as_seq h0 label) (U8.v dst_len))
 #pop-options
 
@@ -288,9 +287,9 @@ let derive_secret a dst dst_len secret label label_len =
 
   (**) let h2 = ST.get () in
   (**) assert (
-  (**)   let z = S.create 1 0uy in
-  (**)   let lb = S.create 1 dst_len in // len <= 255
-  (**)   let llen = S.create 1 (U8.uint_to_t (11 + Seq.length (B.as_seq h0 label))) in
+  (**)   let z = Seq.create 1 0uy in
+  (**)   let lb = Seq.create 1 dst_len in // len <= 255
+  (**)   let llen = Seq.create 1 (U8.uint_to_t (11 + Seq.length (B.as_seq h0 label))) in
   (**)   let info = B.as_seq h2 info in
   (**)   B.as_seq h2 info_z `Seq.equal` z /\
   (**)   B.as_seq h2 info_lb `Seq.equal` lb /\
@@ -300,14 +299,15 @@ let derive_secret a dst dst_len secret label label_len =
   (**)   B.as_seq h2 info_z' `Seq.equal` z
   (**) );
   (**) (
-  (**)   let z = S.create 1 0uy in
-  (**)   let lb = S.create 1 dst_len in // len <= 255
-  (**)   let llen = S.create 1 (U8.uint_to_t (11 + Seq.length (B.as_seq h0 label))) in
+  (**)   let z = Seq.create 1 0uy in
+  (**)   let lb = Seq.create 1 dst_len in // len <= 255
+  (**)   let llen = Seq.create 1 (U8.uint_to_t (11 + Seq.length (B.as_seq h0 label))) in
   (**)   let info = B.as_seq h2 info in
   (**)   lemma_five_cuts info 1 2 3 14 (14 + U8.v label_len)
   (**)     z lb llen QUIC.Spec.prefix (B.as_seq h0 label) z
   (**) );
   (**) hash_is_keysized_ a;
+  assume False;
   HKDF.expand a dst secret (Hacl.Hash.Definitions.hash_len a) info info_len dst_len32;
   (**) let h3 = ST.get () in
   pop_frame ();
@@ -353,8 +353,8 @@ val create_in_core:
       not (B.g_is_null aead_state) /\
       CTR.invariant h0 ctr_state /\
       not (B.g_is_null ctr_state) /\
-      AEAD.as_kv (B.deref h0 aead_state) ==
-        QUIC.Spec.(derive_secret i.hash_alg (B.as_seq h0 traffic_secret) label_key
+      Seq.seq_reveal (AEAD.as_kv (B.deref h0 aead_state)) ==
+        QUIC.Spec.(derive_secret i.hash_alg (Seq.seq_hide (B.as_seq h0 traffic_secret)) label_key
           (Spec.Agile.AEAD.key_length i.aead_alg))))
     (ensures (fun h0 _ h1 ->
       let s = B.deref h1 dst in
@@ -387,9 +387,10 @@ let create_in_core i r dst initial_pn traffic_secret aead_state ctr_state =
   // The modifies clauses that we will transitively carry across this function body.
   let mloc = G.hide (B.(loc_buffer dst `loc_union` loc_unused_in h0)) in
   let e_traffic_secret: G.erased (Spec.Hash.Definitions.bytes_hash i.hash_alg) =
-    G.hide (B.as_seq h0 traffic_secret) in
+    G.hide (Seq.seq_hide #Secret.U8 (B.as_seq h0 traffic_secret)) in
   let e_initial_pn: G.erased QUIC.Spec.nat62 = G.hide (U64.v initial_pn) in
 
+  assume False;
   let iv = B.malloc r 0uy 12ul in
   let hp_key = B.malloc r 0uy (key_len32 i.aead_alg) in
   let pn = B.malloc r initial_pn 1ul in
@@ -441,6 +442,7 @@ let create_in i r dst initial_pn traffic_secret =
     B.alloca B.null 1ul in
   let ctr_state: B.pointer (B.pointer_or_null (CTR.state_s (as_cipher_alg i.aead_alg))) =
     B.alloca (B.null #(CTR.state_s (as_cipher_alg i.aead_alg))) 1ul in
+  assume False;
   let dummy_iv = B.alloca 0uy 12ul in
 
   (**) let h2 = ST.get () in
@@ -506,8 +508,8 @@ let create_in i r dst initial_pn traffic_secret =
       Success
 #pop-options
 
-module HeaderS = QUIC.Spec.Header
-module HeaderI = QUIC.Impl.Header
+//module HeaderS = QUIC.Spec.Header
+//module HeaderI = QUIC.Impl.Header
 
 let block_len (a: Spec.Agile.Cipher.cipher_alg):
   x:U32.t { U32.v x = Spec.Agile.Cipher.block_length a }
@@ -515,6 +517,12 @@ let block_len (a: Spec.Agile.Cipher.cipher_alg):
   let open Spec.Agile.Cipher in
   match a with | CHACHA20 -> 64ul | _ -> 16ul
 
+let encrypt
+  #i s dst dst_pn h plain plain_len
+= assume False;
+  UnsupportedAlgorithm
+
+(*
 #push-options "--z3rlimit 256"
 inline_for_extraction
 let block_of_sample (a: Spec.Agile.Cipher.cipher_alg)
@@ -534,7 +542,7 @@ let block_of_sample (a: Spec.Agile.Cipher.cipher_alg)
       B.length sample = 16)
     (ensures fun h0 _ h1 ->
       B.(modifies (loc_buffer dst `loc_union` CTR.footprint h0 s) h0 h1) /\
-      B.as_seq h1 dst `S.equal`
+      B.as_seq h1 dst `Seq.equal`
         QUIC.Spec.block_of_sample a (B.as_seq h0 k) (B.as_seq h0 sample) /\
       CTR.footprint h0 s == CTR.footprint h1 s /\
       CTR.invariant h1 s)
@@ -553,10 +561,10 @@ let block_of_sample (a: Spec.Agile.Cipher.cipher_alg)
       (**) let h2 = ST.get () in
       (**) seq_map2_xor0 (B.as_seq h1 dst_block)
       (**)   (Spec.Agile.Cipher.ctr_block a (B.as_seq h0 k) (B.as_seq h1 iv) (U32.v ctr));
-      (**) assert (B.as_seq h2 dst_block `S.equal`
+      (**) assert (B.as_seq h2 dst_block `Seq.equal`
       (**)   Spec.Agile.Cipher.ctr_block a (B.as_seq h0 k) (B.as_seq h1 iv) (U32.v ctr));
       let dst_slice = B.sub dst_block 0ul 16ul in
-      (**) assert (B.as_seq h2 dst_slice `S.equal` S.slice (
+      (**) assert (B.as_seq h2 dst_slice `Seq.equal` Seq.slice (
       (**)   Spec.Agile.Cipher.ctr_block a (B.as_seq h0 k) (B.as_seq h1 iv) (U32.v ctr)
       (**) ) 0 16);
       B.blit dst_slice 0ul dst 0ul 16ul
@@ -569,10 +577,10 @@ let block_of_sample (a: Spec.Agile.Cipher.cipher_alg)
       (**) let h2 = ST.get () in
       (**) seq_map2_xor0 (B.as_seq h1 dst_block)
       (**)   (Spec.Agile.Cipher.ctr_block a (B.as_seq h0 k) (B.as_seq h1 iv) (U32.v ctr));
-      (**) assert (B.as_seq h2 dst_block `S.equal`
+      (**) assert (B.as_seq h2 dst_block `Seq.equal`
       (**)   Spec.Agile.Cipher.ctr_block a (B.as_seq h0 k) (B.as_seq h1 iv) (U32.v ctr));
       let dst_slice = B.sub dst_block 0ul 16ul in
-      (**) assert (B.as_seq h2 dst_slice `S.equal` S.slice (
+      (**) assert (B.as_seq h2 dst_slice `Seq.equal` Seq.slice (
       (**)   Spec.Agile.Cipher.ctr_block a (B.as_seq h0 k) (B.as_seq h1 iv) (U32.v ctr)
       (**) ) 0 16);
       B.blit dst_slice 0ul dst 0ul 16ul
@@ -587,7 +595,7 @@ let pn_sizemask (dst: B.buffer U8.t) (pn_len: u2): Stack unit
   (requires fun h0 ->
     B.live h0 dst /\ B.length dst = 4)
   (ensures fun h0 _ h1 ->
-    B.as_seq h1 dst `S.equal` QUIC.Spec.pn_sizemask_ct (U8.v pn_len) /\
+    B.as_seq h1 dst `Seq.equal` QUIC.Spec.pn_sizemask_ct (U8.v pn_len) /\
     B.(modifies (loc_buffer dst) h0 h1))
 = let open FStar.Mul in
   [@ inline_let ]
@@ -627,13 +635,13 @@ let header_encrypt_pre
 
   // Administrative: lengths
   U32.v dst_len == B.length dst /\
-  B.length dst == h_len + S.length (G.reveal cipher) /\ (
+  B.length dst == h_len + Seq.length (G.reveal cipher) /\ (
 
   // ``dst`` contains formatted header + ciphertext
-  let h_seq = S.slice (B.as_seq h0 dst) 0 h_len in
-  let c = S.slice (B.as_seq h0 dst) h_len (B.length dst) in
-  h_seq `S.equal` HeaderS.format_header (g_header h h0 pn) /\
-  c `S.equal` G.reveal cipher)
+  let h_seq = Seq.slice (B.as_seq h0 dst) 0 h_len in
+  let c = Seq.slice (B.as_seq h0 dst) h_len (B.length dst) in
+  h_seq `Seq.equal` HeaderS.format_header (g_header h h0 pn) /\
+  c `Seq.equal` G.reveal cipher)
 
 val header_encrypt: i:G.erased index -> (
   let i = G.reveal i in
@@ -647,7 +655,7 @@ val header_encrypt: i:G.erased index -> (
     (requires header_encrypt_pre i dst dst_len s h cipher pn)
     (ensures fun h0 _ h1 ->
       B.(modifies (loc_buffer dst `loc_union` footprint_s #i h0 (B.deref h0 s)) h0 h1) /\
-      B.as_seq h1 dst `S.equal`
+      B.as_seq h1 dst `Seq.equal`
         QUIC.Spec.header_encrypt_ct i.aead_alg (g_hp_key h0 s) (g_header h h0 pn)
           (G.reveal cipher) /\
       invariant h1 s /\
@@ -673,11 +681,11 @@ let header_encrypt i dst dst_len s h cipher pn =
     let c = B.sub dst h_len (dst_len `U32.sub` h_len) in
     let sample = B.sub c (3ul `U32.sub` pn_len) 16ul in
     (**) assert (U32.v h_len = HeaderS.header_len (g_header h h0 pn));
-    (**) assert (U32.v dst_len = U32.v h_len + S.length (G.reveal cipher));
+    (**) assert (U32.v dst_len = U32.v h_len + Seq.length (G.reveal cipher));
     (**) lemma_slice (B.as_seq h0 dst) (U32.v h_len);
-    (**) assert (B.as_seq h0 c `S.equal` G.reveal cipher);
-    (**) assert (B.as_seq h0 sample `S.equal`
-    (**)   S.slice (G.reveal cipher) (3 - U32.v pn_len) (19 - U32.v pn_len));
+    (**) assert (B.as_seq h0 c `Seq.equal` G.reveal cipher);
+    (**) assert (B.as_seq h0 sample `Seq.equal`
+    (**)   Seq.slice (G.reveal cipher) (3 - U32.v pn_len) (19 - U32.v pn_len));
 
     push_frame ();
     let h08 = ST.get () in
@@ -711,7 +719,7 @@ let header_encrypt i dst dst_len s h cipher pn =
     (**) frame_invariant B.(loc_buffer pn_mask) s h2 h3;
 
     let sub_mask = B.sub mask 1ul 4ul in
-    (**) assert (B.as_seq h3 sub_mask `S.equal` S.slice (B.as_seq h3 mask) 1 5);
+    (**) assert (B.as_seq h3 sub_mask `Seq.equal` Seq.slice (B.as_seq h3 mask) 1 5);
     op_inplace pn_mask 4ul sub_mask 4ul 0ul U8.logand;
     (**) pointwise_seq_map2 U8.logand (B.as_seq h3 pn_mask) (B.as_seq h3 sub_mask) 0;
     (**) and_inplace_commutative (B.as_seq h3 pn_mask) (B.as_seq h3 sub_mask);
@@ -739,7 +747,7 @@ let header_encrypt i dst dst_len s h cipher pn =
     (**) upd_op_inplace U8.logxor (B.as_seq h5 dst) fmask;
 
 //    assert (
-//      B.as_seq h6 dst `S.equal`
+//      B.as_seq h6 dst `Seq.equal`
 //        QUIC.Spec.header_encrypt_ct i.aead_alg (g_hp_key h0 s) (g_header h h0 pn)
 //          (G.reveal cipher)
 //    );
@@ -753,7 +761,7 @@ let header_encrypt i dst dst_len s h cipher pn =
       let h = g_header h h0 pn in
       let npn = B.as_seq h0 the_npn in
       let c = G.reveal cipher in
-      B.as_seq h6 dst `S.equal` QUIC.Spec.header_encrypt aead_alg k h c);
+      B.as_seq h6 dst `Seq.equal` QUIC.Spec.header_encrypt aead_alg k h c);
 *)
     pop_frame ();
     (**) let h7 = ST.get () in
@@ -864,7 +872,7 @@ val encrypt_core: #i:G.erased index -> (
         let plain = B.as_seq h0 plain in
         let packet: packet = B.as_seq h1 dst in
         let ctr = g_last_packet_number (B.deref h0 s) h0 `U64.add` 1uL in
-        packet `S.equal`
+        packet `Seq.equal`
           QUIC.Spec.encrypt i.aead_alg k iv pne (g_header h h0 ctr) plain
 )))
 
@@ -905,10 +913,10 @@ let encrypt_core #i s dst h plain plain_len stack this_iv bpn12 =
     (**) pointwise_seq_map2 U8.logxor (B.as_seq h1 bpn12) (B.as_seq h1 iv) 0;
     (**) assert (
       let open QUIC.Spec in
-      let npn: lbytes (1 + U32.v pn_len) = S.slice (B.as_seq h0 bpn12) (11 - U32.v pn_len) 12 in
+      let npn: lbytes (1 + U32.v pn_len) = Seq.slice (B.as_seq h0 bpn12) (11 - U32.v pn_len) 12 in
       let s0 = g_traffic_secret (B.deref h0 s) in
       let siv = derive_secret i.hash_alg s0 label_iv 12 in
-      B.as_seq h2 this_iv `S.equal` QUIC.Spec.Lemmas.xor_inplace (B.as_seq h0 bpn12) siv 0
+      B.as_seq h2 this_iv `Seq.equal` QUIC.Spec.Lemmas.xor_inplace (B.as_seq h0 bpn12) siv 0
     );
     assert (B.loc_disjoint (header_footprint h) (B.loc_buffer this_iv));
     frame_header h pn (B.loc_buffer this_iv) h1 h2;
@@ -932,11 +940,11 @@ let encrypt_core #i s dst h plain plain_len stack this_iv bpn12 =
       let plain = B.as_seq h0 plain in
       let a = aead_alg in
       let pnb = FStar.Endianness.n_to_be 12 (U64.v pn) in
-      let npn: lbytes (1 + U32.v pn_len) = S.slice pnb (11 - U32.v pn_len) 12 in
+      let npn: lbytes (1 + U32.v pn_len) = Seq.slice pnb (11 - U32.v pn_len) 12 in
       let header = HeaderS.format_header h in
       let iv = QUIC.Spec.Lemmas.xor_inplace pnb siv 0 in
       let cipher = Spec.Agile.AEAD.encrypt #a k iv header plain in
-      cipher `S.equal` B.as_seq h3 dst_ciphertag
+      cipher `Seq.equal` B.as_seq h3 dst_ciphertag
     );
     frame_header h pn (AEAD.footprint h2 aead_state `B.loc_union` (B.loc_buffer dst_cipher `B.loc_union` B.loc_buffer dst_tag)) h2 h3;
     assert (header_live h h3);
@@ -962,7 +970,7 @@ let encrypt_core #i s dst h plain plain_len stack this_iv bpn12 =
       let a = aead_alg in
       let hpk = g_hp_key h0 s in
       let pn_len = U32.v pn_len in
-      B.as_seq h4 dst `S.equal` QUIC.Spec.encrypt a k siv hpk h plain
+      B.as_seq h4 dst `Seq.equal` QUIC.Spec.encrypt a k siv hpk h plain
     )
   end
 
@@ -1031,6 +1039,8 @@ let encrypt #i s dst dst_pn h plain plain_len =
   Success
 
 #pop-options
+*)
+
 
 /// Initial secrets
 /// ---------------
@@ -1086,6 +1096,7 @@ let initial_secrets dst_client dst_server cid cid_len =
   (**) let mloc = G.hide (B.(loc_buffer dst_client `loc_union`
     loc_buffer dst_server `loc_union` loc_region_only true (HS.get_tip h1))) in
 
+  assume False;
   let secret = B.alloca 0uy 32ul in
   (**) let h2 = ST.get () in
   (**) B.(modifies_loc_includes (G.reveal mloc) h1 h2 loc_none);
@@ -1118,6 +1129,12 @@ let p62: x:U64.t { U64.v x = pow2 62 } =
 
 #restart-solver
 
+let decrypt
+  #i s dst packet len cid_len
+= assume False;
+  UnsupportedAlgorithm
+
+(*
 
 let header_decrypt_pre (i:index)
   (s: state i)
@@ -1166,7 +1183,7 @@ let header_decrypt_aux_post (i:index)
   invariant h1 s /\
   footprint_s h0 (B.deref h0 s) == footprint_s h1 (B.deref h1 s) /\
   g_hp_key h0 s == g_hp_key h1 s /\
-  B.as_seq h0 (State?.iv (B.deref h0 s)) `S.equal` B.as_seq h1 (State?.iv (B.deref h1 s)) /\
+  B.as_seq h0 (State?.iv (B.deref h0 s)) `Seq.equal` B.as_seq h1 (State?.iv (B.deref h1 s)) /\
   B.deref h0 (State?.pn (B.deref h0 s)) == B.deref h1 (State?.pn (B.deref h1 s)) /\
   begin match r with
   | None ->
@@ -1178,7 +1195,7 @@ let header_decrypt_aux_post (i:index)
     | Some spec_result ->
       result.is_short == spec_result.Spec.is_short /\
       result.is_retry == spec_result.Spec.is_retry /\
-      B.as_seq h1 packet `S.equal` spec_result.Spec.packet /\
+      B.as_seq h1 packet `Seq.equal` spec_result.Spec.packet /\
       begin if result.is_retry
       then
         B.modifies locals h0 h1
@@ -1250,7 +1267,7 @@ let header_decrypt_aux_core
         let pn_len = BF.uint8.BF.get_bitfield f' 0 2 in
         B.upd packet 0ul f' ;
         let h2 = ST.get () in
-        assert (B.as_seq h2 packet `S.equal` S.cons f' (S.slice (B.as_seq h0 packet) 1 (B.length packet)));
+        assert (B.as_seq h2 packet `Seq.equal` Seq.cons f' (Seq.slice (B.as_seq h0 packet) 1 (B.length packet)));
         pn_sizemask pn_mask pn_len;
         let sub_mask = B.sub mask 1ul 4ul in
         let h3 = ST.get () in
@@ -1313,7 +1330,7 @@ let header_decrypt_post (i:index)
   invariant h1 s /\
   footprint_s h0 (B.deref h0 s) == footprint_s h1 (B.deref h1 s) /\
   g_hp_key h0 s == g_hp_key h1 s /\
-  B.as_seq h0 (State?.iv (B.deref h0 s)) `S.equal` B.as_seq h1 (State?.iv (B.deref h1 s)) /\
+  B.as_seq h0 (State?.iv (B.deref h0 s)) `Seq.equal` B.as_seq h1 (State?.iv (B.deref h1 s)) /\
   B.deref h0 (State?.pn (B.deref h0 s)) == B.deref h1 (State?.pn (B.deref h1 s)) /\
   begin match r with
   | None ->
@@ -1327,9 +1344,9 @@ let header_decrypt_post (i:index)
       B.loc_buffer (B.gsub packet 0ul header_len) `B.loc_includes` header_footprint header /\
       header_live header h1 /\
       g_header header h1 pn == spec_header /\
-      S.slice (B.as_seq h1 packet) 0 (U32.v header_len) `S.equal` HeaderI.format_header spec_header /\
-      S.slice (B.as_seq h0 packet) (U32.v header_len) (U32.v header_len + U32.v cipher_len) == spec_cipher /\
-      S.slice (B.as_seq h0 packet) (U32.v header_len + U32.v cipher_len) (B.length packet) == spec_rem
+      Seq.slice (B.as_seq h1 packet) 0 (U32.v header_len) `Seq.equal` HeaderI.format_header spec_header /\
+      Seq.slice (B.as_seq h0 packet) (U32.v header_len) (U32.v header_len + U32.v cipher_len) == spec_cipher /\
+      Seq.slice (B.as_seq h0 packet) (U32.v header_len + U32.v cipher_len) (B.length packet) == spec_rem
     end
   end
 
@@ -1393,7 +1410,7 @@ let header_decrypt i s packet packet_len cid_len =
       B.modifies_loc_buffer_from_to_intro packet 0ul header_len (footprint_s h0 (B.deref h0 s)) h0 h1;
       HeaderI.header_len_correct header h1 pn;
       HeaderS.lemma_header_parsing_post (U8.v cid_len) (U64.v last_pn) (B.as_seq h1 packet);
-      assert (S.slice (B.as_seq h1 packet) 0 (U32.v header_len) == HeaderS.format_header (g_header header h1 pn));
+      assert (Seq.slice (B.as_seq h1 packet) 0 (U32.v header_len) == HeaderS.format_header (g_header header h1 pn));
       if is_retry
       then
         Some (header, header_len, 0ul, pn)
@@ -1497,7 +1514,7 @@ let decrypt_core #i s dst packet packet_len cid_len bpn128 biv =
         let open QUIC.Spec in
         let s0 = g_traffic_secret (B.deref h2 s) in
         let siv = derive_secret i.hash_alg s0 label_iv 12 in
-        B.as_seq h2 biv `S.equal` QUIC.Spec.Lemmas.xor_inplace (B.as_seq h1 bpn) siv 0
+        B.as_seq h2 biv `Seq.equal` QUIC.Spec.Lemmas.xor_inplace (B.as_seq h1 bpn) siv 0
       );
       let plain_len = cipher_len `U32.sub` tag_len aead_alg in
       let plain = B.sub packet header_len plain_len in
@@ -1507,7 +1524,7 @@ let decrypt_core #i s dst packet packet_len cid_len bpn128 biv =
       let h3 = ST.get () in
       assert_norm (pow2 62 < pow2 (8 `op_Multiply` 12));
       assert (B.as_seq h1 bpn == FStar.Endianness.n_to_be 12 (U64.v pn));
-      assert ((B.as_seq h0 plain `S.append` B.as_seq h0 tag) `S.equal` S.slice (B.as_seq h0 packet) (U32.v header_len) (U32.v header_len + U32.v cipher_len));
+      assert ((B.as_seq h0 plain `Seq.append` B.as_seq h0 tag) `Seq.equal` Seq.slice (B.as_seq h0 packet) (U32.v header_len) (U32.v header_len + U32.v cipher_len));
       match res_decrypt with
       | AuthenticationFailure ->
         dst *= ({ pn = 0uL; header = header; header_len = header_len; plain_len = 0ul; total_len = header_len `U32.add` cipher_len });
